CollapsingTowers/TwoLevel/Basic.lean
@@ -23,6 +23,7 @@ inductive Expr : Type where
   | lets (b : Expr) (e : Expr)
   | let𝕔 (b : Expr) (e : Expr)
   | loc (n : ℕ)
+  | load₁ (e : Expr)
 
 abbrev TEnv :=
   List Ty
