CollapsingTowers/TwoLevel/Shift.lean
@@ -19,6 +19,7 @@ def shiftl_at (x : ℕ) (n : ℕ) : Expr -> Expr
   | .lets b e => .lets (shiftl_at x n b) (shiftl_at x n e)
   | .let𝕔 b e => .let𝕔 (shiftl_at x n b) (shiftl_at x n e)
   | .loc n => .loc n
+  | .load₁ e => .load₁ (shiftl_at x n e)
 
 theorem shiftl_opening :
     ∀ x y e n i, x <= y -> shiftl_at x n (opening i (.fvar y) e) = opening i (.fvar (y + n)) (shiftl_at x n e) :=
@@ -46,7 +47,8 @@ theorem shiftl_opening :
   | lam𝕔 _ IH
   | code _ IH
   | reflect _ IH
-  | lit₂ _ IH =>
+  | lit₂ _ IH
+  | load₁ _ IH =>
     simp; apply IH
 
 theorem shiftl_open₀ : ∀ x y e n, x <= y -> shiftl_at x n (open₀ y e) = open₀ (y + n) (shiftl_at x n e) := by
@@ -77,7 +79,8 @@ theorem shiftl_closed_at :
   | lam𝕔 _ IH
   | code _ IH
   | reflect _ IH
-  | lit₂ _ IH =>
+  | lit₂ _ IH
+  | load₁ _ IH =>
     simp; apply IH; apply Hclose
 
 theorem shiftl_id :
@@ -102,7 +105,8 @@ theorem shiftl_id :
   | lam𝕔 _ IH
   | code _ IH
   | reflect _ IH
-  | lit₂ _ IH =>
+  | lit₂ _ IH
+  | load₁ _ IH =>
     simp; apply IH
 
 @[simp]
@@ -123,6 +127,7 @@ def shiftr_at (x : ℕ) : Expr -> Expr
   | .lets b e => .lets (shiftr_at x b) (shiftr_at x e)
   | .let𝕔 b e => .let𝕔 (shiftr_at x b) (shiftr_at x e)
   | .loc n => .loc n
+  | .load₁ e => .load₁ (shiftr_at x e)
 
 theorem shiftr_opening :
     ∀ x y e i, x < y -> shiftr_at x (opening i (.fvar y) e) = opening i (.fvar (y - 1)) (shiftr_at x e) :=
@@ -150,7 +155,8 @@ theorem shiftr_opening :
   | lam𝕔 _ IH
   | code _ IH
   | reflect _ IH
-  | lit₂ _ IH =>
+  | lit₂ _ IH
+  | load₁ _ IH =>
     simp; apply IH
 
 theorem shiftr_open₀ : ∀ x y e, x < y -> shiftr_at x (open₀ y e) = open₀ (y - 1) (shiftr_at x e) :=
@@ -182,7 +188,8 @@ theorem shiftr_closed_at : ∀ x y e, y < x -> closed_at e (x + 1) -> closed_at 
   | lam𝕔 _ IH
   | code _ IH
   | reflect _ IH
-  | lit₂ _ IH =>
+  | lit₂ _ IH
+  | load₁ _ IH =>
     simp; apply IH; apply Hclose
 
 theorem shiftr_closed_at_id : ∀ x e, closed_at e x -> closed_at (shiftr_at x e) x :=
@@ -209,7 +216,8 @@ theorem shiftr_closed_at_id : ∀ x e, closed_at e x -> closed_at (shiftr_at x e
   | lam𝕔 _ IH
   | code _ IH
   | reflect _ IH
-  | lit₂ _ IH =>
+  | lit₂ _ IH
+  | load₁ _ IH =>
     simp; apply IH; apply Hclose
 
 theorem shiftr_id :
@@ -234,5 +242,6 @@ theorem shiftr_id :
   | lam𝕔 _ IH
   | code _ IH
   | reflect _ IH
-  | lit₂ _ IH =>
+  | lit₂ _ IH
+  | load₁ _ IH =>
     simp; apply IH
